a few comments and cleanup

src/ml/main.ml
@@ -32,7 +32,7 @@ let test_pp_dir dir =
 
 (* Use the --test option to run unit tests and the quit the program. *)
 let args =
-  [ ("--test", Unit exec_tests, "run the test suite, ignoring other inputs")
+  [ ("--test", Unit exec_tests, "run the test suite, ignoring later inputs")
   ; ("--test-pp-dir", String test_pp_dir, "run the parsing/pretty-printing tests on all .ll files in the given directory")
   ; ("-op", Set_string Platform.output_path, "set the path to the output files directory  [default='output']")
   ; ("-interpret", Set Driver.interpret, "interpret ll program starting from 'main'")
