src/coq/StepSemanticsProp.v
@@ -11,7 +11,7 @@
 Require Import ZArith List String Omega.
 Require Import  Vellvm.Classes Vellvm.Util.
 Require Import Vellvm.LLVMAst Vellvm.AstLib Vellvm.CFG Vellvm.CFGProp.
-Require Import Vellvm.StepSemantics.
+Require Import Vellvm.LLVMIO Vellvm.StepSemantics.
 
 Import ListNotations.
 
@@ -21,8 +21,119 @@ Set Contextual Implicit.
 
 
 Module StepSemanticsProp(A:ADDR).
+  Module SS := StepSemantics(A).
+  Import SS.
+  Import SS.DV.
+
+Section Properties.
+(* environment facts -------------------------------------------------------- 
+  Lemma lookup_env_hd : forall id dv e, lookup_env (add_env id dv e) id = Ret dv.
+  Proof.
+    intros id dv e.  unfold lookup_env. 
+    unfold add_env.
+    apply ENV.find_1. apply ENV.add_1. reflexivity.
+  Qed.  
+
+  Lemma lookup_env_tl : forall id1 v1 e id2,
+      id1 <> id2 -> lookup_env (add_env id1 v1 e) id2 = lookup_env e id2.
+  Proof.
+    unfold lookup_env.
+    intros id1 v1 e id2 H.
+    unfold add_env. 
+    remember (ENV.find (elt:=value) id2 (ENV.add id1 v1 e)) as x.
+    remember (ENV.find (elt:=value) id2 e) as y.
+    destruct x; destruct y; auto.
+    - symmetry in Heqx. rewrite <- ENVFacts.find_mapsto_iff in Heqx.
+      symmetry in Heqy. rewrite <- ENVFacts.find_mapsto_iff in Heqy.
+      rewrite ENVFacts.add_neq_mapsto_iff in Heqx; auto.
+      assert (v = v0). { eapply ENVFacts.MapsTo_fun; eauto. }
+                       subst; reflexivity.                 
+    - symmetry in Heqx. rewrite <- ENVFacts.find_mapsto_iff in Heqx.
+      symmetry in Heqy. rewrite <- ENVFacts.not_find_in_iff in Heqy.
+      rewrite ENVFacts.add_neq_mapsto_iff in Heqx; auto.
+      unfold ENV.In in Heqy. unfold ENV.Raw.In0 in Heqy. assert False. apply Heqy. exists v. apply Heqx. destruct H0.
+    - symmetry in Heqx. rewrite <- ENVFacts.not_find_in_iff in Heqx.
+      symmetry in Heqy. rewrite <- ENVFacts.find_mapsto_iff in Heqy.
+      assert False. apply Heqx. unfold ENV.In.  unfold ENV.Raw.In0. exists v. apply ENV.add_2; auto. destruct H0.
+  Qed.  
 
 
+  Lemma lookup_add_env_inv :
+    forall id1 v e id2 u
+      (Hl: lookup_env (add_env id1 v e) id2 = Some u),
+      (id1 = id2 /\ v = u) \/ (id1 <> id2 /\ lookup_env e id2 = Some u).
+  Proof.
+    intros id1 v e id2 u Hl.
+    unfold add_env in Hl.
+    unfold lookup_env in *.
+    rewrite <- ENVFacts.find_mapsto_iff in Hl.
+    apply ENVFacts.add_mapsto_iff in Hl.
+    destruct Hl as [H | H].
+    - left. assumption.
+    - right. rewrite <- ENVFacts.find_mapsto_iff. assumption.
+  Qed.      
+ *)
+  
+  Definition pc_satisfies (CFG:mcfg) (p:pc) (P:cmd -> Prop) : Prop :=
+    forall cmd, fetch CFG p = Some cmd -> P cmd.
+
+
+  (* Move to AstLib.v ? *)
+  Definition is_Op (i:instr) : Prop :=
+    match i with
+    | INSTR_Op _ => True
+    | _ => False
+    end.
+
+  Definition is_Eff (i:instr) : Prop :=
+    match i with 
+    | INSTR_Alloca t nb a => True
+    | INSTR_Load v t p a => True
+    | INSTR_Store v val p a => True
+    | _ => False    (* TODO: Think about call *)
+    end.
+  
+  Definition is_Call (i:instr) : Prop :=
+    match i with
+    | INSTR_Call _ _ => True
+    | _ => False
+    end.
+  
+  Definition pc_non_call (CFG:mcfg) (p:pc) : Prop :=
+    pc_satisfies CFG p (fun c => exists i, not (is_Call i) /\ c = Inst i).
+
+  Ltac step_destruct :=
+    repeat (match goal with
+            | [ H : context[do _ <- trywith _ ?E; _] |- _ ] => destruct E; [simpl in H | solve [inversion H]]
+            | [ H : context[do _ <- ?E; _] |- _ ] => destruct E; [solve [inversion H] | simpl in H]
+            | [ H : context[match ?E with _ => _ end] |- _ ] => destruct E; try solve [inversion H]; simpl in H
+            | [ H : Step (?p, _ , _) = Step (?q, _, _) |- Some ?p = Some ?q ] => inversion H; auto
+            | [ H : ~ (is_Call (INSTR_Call _ _)) |- _ ] => simpl in H; contradiction
+            end).
+
+  (* Not true for Call *)
+  (*
+  Lemma step_pc_incr_inversion:
+    forall CFG pc1 e1 k1 pc2 e2 k2
+      (Hpc: pc_non_call CFG pc1)
+      (Hstep: step CFG (pc1, e1, k1) = Step (pc2, e2, k2)),
+      incr_pc CFG pc1 = Some pc2.
+  Proof.
+    (*
+    intros CFG pc1 e1 k1 pc2 e2 k2 Hpc Hstep.
+    simpl in Hstep.
+    unfold pc_non_call in Hpc. unfold pc_satisfies in Hpc.
+    destruct (fetch CFG pc1); try solve [inversion Hstep]; simpl in Hstep.
+    specialize Hpc with (cmd0 := c). destruct Hpc as [i [Hi Hc]]; auto.
+    subst.
+    destruct (incr_pc CFG pc1); [simpl in Hstep | solve [inversion Hstep]].
+    step_destruct.*)
+    admit. (* TODO: fix up once the effects interface is stabilized *)
+  Admitted.
+*)
+End Properties.
+
+  
   (*
   Lemma stepD_Op_inversion :
     forall CFG fn bid phis term,
